@prefix : <https://w3id.org/def/didl#> .
@prefix dc: <http://purl.org/dc/elements/1.1/> .
@prefix owl: <http://www.w3.org/2002/07/owl#> .
@prefix rdf: <http://www.w3.org/1999/02/22-rdf-syntax-ns#> .
@prefix sec: <https://w3id.org/security#> .
@prefix xsd: <http://www.w3.org/2001/XMLSchema#> .
@prefix cred: <https://www.w3.org/ns/credentials#> .
@prefix dedl: <https://w3id.org/def/dedl#> .
@prefix didl: <https://w3id.org/def/didl#> .
@prefix foaf: <http://xmlns.com/foaf/0.1/> .
@prefix rdfs: <http://www.w3.org/2000/01/rdf-schema#> .
@prefix dcterms: <http://purl.org/dc/terms/> .
@base <https://w3id.org/def/didl#> .

<https://w3id.org/def/didl> rdf:type owl:Ontology ;
                             dc:creator "Jiahang Chen"@en ;
                             dc:description "The Digital Identity Description Language (DIDL) is an abstract language to describe identity concepts used in data ecosystems. The core component, identity, is specialized into identifiers, credentials, and assertions in this language, contributing to authentication and authorization."@en ;
                             dc:title "DIDL Vocabulary & Expression 0.1"@en ;
                             dcterms:abstract """The DIDL is a description language to represent diverse identity con-
cepts, ensuring technical and semantic compatibility across different data ecosystems."""@en ;
                             dcterms:created "2025-04-29T00:00:00"^^xsd:dateTime ;
                             dcterms:license "http://creativecommons.org/licenses/by/4.0/" ;
                             rdfs:comment "This is a vocabulary for DIDL Version 0.1"@en ;
                             rdfs:label "DIDL" ;
                             owl:versionInfo 0.1 .

#################################################################
#    Annotation properties
#################################################################

###  http://purl.org/dc/elements/1.1/creator
dc:creator rdf:type owl:AnnotationProperty ;
           rdfs:comment "This individual represents creator." ;
           rdfs:label "creator" .


###  http://purl.org/dc/elements/1.1/description
dc:description rdf:type owl:AnnotationProperty ;
               rdfs:comment "This individual represents description." ;
               rdfs:label "description" .


###  http://purl.org/dc/elements/1.1/title
dc:title rdf:type owl:AnnotationProperty ;
         rdfs:comment "This individual represents title." ;
         rdfs:label "title".


###  http://purl.org/dc/terms/abstract
dcterms:abstract rdf:type owl:AnnotationProperty .


###  http://purl.org/dc/terms/created
dcterms:created rdf:type owl:AnnotationProperty ;
                rdfs:comment "This individual represents created." ;
                rdfs:label "created" .


###  http://purl.org/dc/terms/license
dcterms:license rdf:type owl:AnnotationProperty ;
                rdfs:comment "This individual represents license.";
                rdfs:label "license".


#################################################################
#    Object Properties
#################################################################

###  http://purl.org/dc/elements/1.1/identifier
dc:identifier rdf:type owl:ObjectProperty ;
              owl:equivalentProperty didl:identifier ;
              rdfs:comment "This property represents an unambiguous reference to a resource within a given context."@en ;
              rdfs:label "identifier"@en .


###  https://w3id.org/def/didl#accessCapability
didl:accessCapability rdf:type owl:ObjectProperty ;
                      rdfs:domain didl:Assertion ;
                      rdfs:range didl:AccessCapability ;
                      rdfs:comment "Indicates that an assertion has associated access capabilities"@en ;
                      rdfs:label "accessCapability"@en .


###  https://w3id.org/def/didl#assertedAttribute
didl:assertedAttribute rdf:type owl:ObjectProperty ;
                       rdfs:domain didl:Assertion ;
                       rdfs:range didl:Attribute ;
                       rdfs:comment "Indicates that an assertion has asserted attribute(s)"@en ;
                       rdfs:label "assertedAttribute"@en .


###  https://w3id.org/def/didl#assertion
didl:assertion rdf:type owl:ObjectProperty ;
               rdfs:domain didl:IdentitySubject ;
               rdfs:range didl:Assertion ;
               rdfs:comment "Indicates that an identity subject (i.e., entity) has assertion(s)"@en ;
               rdfs:label "assertion"@en .


###  https://w3id.org/def/didl#assertionFormat
didl:assertionFormat rdf:type owl:ObjectProperty ;
                     rdfs:domain didl:Assertion ;
                     rdfs:range didl:AssertionFormat ;
                     rdfs:comment "Indicates that an assertion has its specific format"@en ;
                     rdfs:label "assertionFormat"@en .


###  https://w3id.org/def/didl#controlledBy
didl:controlledBy rdf:type owl:ObjectProperty ;
                  owl:inverseOf didl:controls ;
                  rdfs:domain didl:Identity ;
                  rdfs:range didl:IdentitySubject ;
                  rdfs:comment "Indicates an identity is controlled by an identity subject (i.e., entity)"@en ;
                  rdfs:label "controlledBy"@en .


###  https://w3id.org/def/didl#controls
didl:controls rdf:type owl:ObjectProperty ;
              rdfs:domain didl:IdentitySubject ;
              rdfs:range didl:Identity ;
              rdfs:comment "Indicates that an identity subject (i.e., entity) controlls an identity"@en ;
              rdfs:label "controls"@en .


###  https://w3id.org/def/didl#credential
didl:credential rdf:type owl:ObjectProperty ;
                rdfs:domain didl:IdentitySubject ;
                rdfs:range didl:Credential ;
                rdfs:comment "Indicates that an identity subject (i.e., entity) has credential(s)."@en ;
                rdfs:label "credential"@en .


###  https://w3id.org/def/didl#credentialAttribute
didl:credentialAttribute rdf:type owl:ObjectProperty ;
                         rdfs:domain didl:Credential ;
                         rdfs:range didl:Attribute ;
                         rdfs:comment "Indicates that a credential has attribute(s) to describe a credential, e.g., username/password"@en ;
                         rdfs:label "credentialAttribute"@en .


###  https://w3id.org/def/didl#credentialFormat
didl:credentialFormat rdf:type owl:ObjectProperty ;
                      rdfs:subPropertyOf owl:topObjectProperty ;
                      rdfs:domain didl:Credential ;
                      rdfs:range didl:CredentialFormat ;
                      rdfs:comment "Indicates that a credential has its specific format"@en ;
                      rdfs:label "credentialFormat"@en .


###  https://w3id.org/def/didl#functional
didl:functional rdf:type owl:ObjectProperty ;
                rdfs:domain didl:Identifier ;
                rdfs:range didl:IdentifierFunctional ;
                rdfs:comment "Indicates that an identifier has its own application-specific use"@en ;
                rdfs:label "functional"@en .


###  https://w3id.org/def/didl#identifier
didl:identifier rdf:type owl:ObjectProperty ;
                rdfs:domain didl:IdentitySubject ;
                rdfs:range didl:Identifier ;
                rdfs:comment "Indicates that an identity subject (i.e., entity) has identifier(s)"@en ;
                rdfs:label "identifier"@en .


###  https://w3id.org/def/didl#identifierFormat
didl:identifierFormat rdf:type owl:ObjectProperty ;
                      rdfs:domain didl:Identifier ;
                      rdfs:range didl:IdentifierFormat ;
                      rdfs:comment "Indicates that an identifier has its specific format"@en ;
                      rdfs:label "identifierFormat"@en .


###  https://w3id.org/def/didl#includesAssertion
didl:includesAssertion rdf:type owl:ObjectProperty ;
                       rdfs:domain didl:AssertionCollection ;
                       rdfs:range didl:Assertion ;
                       rdfs:comment "Indicates the constituent assertion of an assertion collection"@en ;
                       rdfs:label "includesAssertion"@en .


###  https://w3id.org/def/didl#includesIdentifier
didl:includesIdentifier rdf:type owl:ObjectProperty ;
                        rdfs:domain didl:CompositeIdentifier ;
                        rdfs:range didl:Identifier ;
                        rdfs:comment "Indicates the local part of a composite identifier"@en ;
                        rdfs:label "includesIdentifier"@en .


###  https://w3id.org/def/didl#key
didl:key rdf:type owl:ObjectProperty ;
         rdfs:domain didl:Attribute ;
         rdfs:range didl:Key ;
         rdfs:comment "Represents a key of an attribute"@en ;
         rdfs:label "key"@en .


###  https://w3id.org/def/didl#proof
didl:proof rdf:type owl:ObjectProperty ;
           rdfs:domain didl:Assertion ;
           rdfs:range sec:Proof ;
           rdfs:comment "Indicates a proof of an assertion, which ensures the integrity and authenticity of the assertion"@en ;
           rdfs:label "proof"@en .


###  https://w3id.org/def/didl#relatesTo
didl:relatesTo rdf:type owl:ObjectProperty ;
               rdfs:domain [ rdf:type owl:Class ;
                             owl:unionOf ( didl:Assertion
                                           didl:Credential
                                         )
                           ] ;
               rdfs:range didl:Identifier ;
               rdfs:comment "Indicates that an assertion or a credential relates to an identifier of an entity"@en ;
               rdfs:label "relatesTo"@en .


###  https://w3id.org/def/didl#status
didl:status rdf:type owl:ObjectProperty ;
            rdfs:domain didl:Identity ;
            rdfs:range didl:Status ;
            rdfs:comment "Indicates the current status of an identity"@en ;
            rdfs:label "status"@en .


###  https://w3id.org/def/didl#supportedAction
didl:supportedAction rdf:type owl:ObjectProperty ;
                     rdfs:domain didl:AccessCapability ;
                     rdfs:range dedl:Action ;
                     rdfs:comment "Indicates the actions supported by an access capability"@en ;
                     rdfs:label "supportedAction"@en .


###  https://w3id.org/def/didl#supportedResource
didl:supportedResource rdf:type owl:ObjectProperty ;
                       rdfs:domain didl:AccessCapability ;
                       rdfs:range dedl:Resource ;
                       rdfs:comment "Indicates the resources supported by an access capability"@en ;
                       rdfs:label "supportedResource"@en .


###  https://w3id.org/def/didl#value
didl:value rdf:type owl:ObjectProperty ;
           rdfs:domain didl:Attribute ;
           rdfs:range didl:Value ;
           rdfs:comment "Represents a value of an attribute"@en ;
           rdfs:label "value"@en .


#################################################################
#    Data properties
#################################################################

###  https://w3id.org/def/didl#issueDate
didl:issueDate rdf:type owl:DatatypeProperty ;
               owl:equivalentProperty cred:issuanceDate ;
               rdfs:domain didl:Identity ;
               rdfs:range xsd:dateTime ;
               rdfs:comment "Indicates the issue date of an identity"@en ;
               rdfs:label "issueDate"@en .


###  https://w3id.org/def/didl#issuer
didl:issuer rdf:type owl:DatatypeProperty ;
            owl:equivalentProperty cred:issuer ;
            rdfs:domain didl:Identity ;
            rdfs:range xsd:anyURI ;
            rdfs:comment "Indicates the issuer of an identity"@en ;
            rdfs:label "issuer"@en .


###  https://w3id.org/def/didl#namespace
didl:namespace rdf:type owl:DatatypeProperty ;
               rdfs:domain didl:Identifier ;
               rdfs:range xsd:string ;
               rdfs:comment "Indicates a namespace of an identifier, representing its definition scope"@en ;
               rdfs:label "namespace"@en .


###  https://w3id.org/def/didl#profile
didl:profile rdf:type owl:DatatypeProperty ;
             rdfs:subPropertyOf owl:topDataProperty ;
             rdfs:domain didl:Identity ;
             rdfs:range xsd:anyURI ;
             rdfs:comment "Indicates an identifier of a DIDL Profile that the identity conforms to"@en ;
             rdfs:label "profile"@en .


###  https://w3id.org/def/didl#renewableTill
didl:renewableTill rdf:type owl:DatatypeProperty ;
                   rdfs:domain didl:Identity ;
                   rdfs:range xsd:dateTime ;
                   rdfs:comment "Indicates that the identity can be renewed until the given time"@en ;
                   rdfs:label "renewableTill"@en .


###  https://w3id.org/def/didl#uid
didl:uid rdf:type owl:DatatypeProperty ;
         rdfs:domain didl:Identity ;
         rdfs:range xsd:anyURI ;
         rdfs:comment "Indicates the unique identifier of an identity itself, e.g., an ID of a verifiable credential"@en ;
         rdfs:label "uid"@en .


###  https://w3id.org/def/didl#validFrom
didl:validFrom rdf:type owl:DatatypeProperty ;
               owl:equivalentProperty cred:validFrom ;
               rdfs:domain didl:Identity ;
               rdfs:range xsd:dateTime ;
               rdfs:comment "Indicates the date from which an identity is valid"@en ;
               rdfs:label "validFrom"@en .


###  https://w3id.org/def/didl#validTo
didl:validTo rdf:type owl:DatatypeProperty ;
             owl:equivalentProperty cred:validTo ;
             rdfs:domain didl:Identity ;
             rdfs:range xsd:dateTime ;
             rdfs:comment "Indicates the date until which an identity is valid"@en ;
             rdfs:label "validTo"@en .


###  https://www.w3.org/ns/credentials#issuanceDate
cred:issuanceDate rdf:type owl:DatatypeProperty ;
                rdfs:comment "The date and time when the credential was issued"@en ;
                rdfs:label "issuanceDate"@en .


###  https://www.w3.org/ns/credentials#issuer
cred:issuer rdf:type owl:DatatypeProperty ;
            rdfs:comment "The entity that issued the credential"@en ;
            rdfs:label "issuer"@en .


###  https://www.w3.org/ns/credentials#validFrom
cred:validFrom rdf:type owl:DatatypeProperty ;
                rdfs:comment "The date and time from which the credential is valid"@en ;
                rdfs:label "validFrom"@en .


###  https://www.w3.org/ns/credentials#validTo
cred:validTo rdf:type owl:DatatypeProperty ;
              rdfs:comment "The date and time until which the credential is valid"@en ;
              rdfs:label "validTo"@en .


#################################################################
#    Classes
#################################################################

###  http://xmlns.com/foaf/0.1/Agent
foaf:Agent rdf:type owl:Class ;
           owl:equivalentClass didl:IdentitySubject ;
           rdfs:comment "An agent is an entity that can perform actions"@en ;
           rdfs:label "Agent"@en .


###  https://w3id.org/def/dedl#Action
dedl:Action rdf:type owl:Class ;
            rdfs:comment "An action that can be performed on a resource"@en ;
            rdfs:label "Action"@en .


###  https://w3id.org/def/dedl#Resource
dedl:Resource rdf:type owl:Class ;
              rdfs:comment "A resource that can be accessed or manipulated"@en ;
              rdfs:label "Resource"@en .


###  https://w3id.org/def/didl#AccessCapability
didl:AccessCapability rdf:type owl:Class ;
                      rdfs:comment "A capability that defines what actions can be performed on which resources"@en ;
                      rdfs:label "AccessCapability"@en .


###  https://w3id.org/def/didl#Assertion
didl:Assertion rdf:type owl:Class ;
               rdfs:subClassOf didl:Identity ;
               owl:disjointWith didl:Credential ,
                                didl:Identifier ;
               rdfs:comment "A collection of identity-related attributes asserted by a trusted party"@en ;
               rdfs:label "Assertion"@en .


###  https://w3id.org/def/didl#AssertionCollection
didl:AssertionCollection rdf:type owl:Class ;
                         rdfs:subClassOf didl:Assertion ;
                         rdfs:comment "A specialized assertion consists of multiple assertions"@en ;
                         rdfs:label "AssertionCollection"@en .


###  https://w3id.org/def/didl#AssertionFormat
didl:AssertionFormat rdf:type owl:Class ;
                     owl:disjointWith didl:CredentialFormat ,
                                      didl:IdentifierFormat ;
                     rdfs:comment "An assertion format that is specified by a standard or a protocol"@en ;
                     rdfs:label "AssertionFormat"@en .


###  https://w3id.org/def/didl#Attribute
didl:Attribute rdf:type owl:Class ;
               rdfs:comment "An identity-related attribute consists of a key-value pair"@en ;
               rdfs:label "Attribute"@en .


###  https://w3id.org/def/didl#CompositeIdentifier
didl:CompositeIdentifier rdf:type owl:Class ;
                         rdfs:subClassOf didl:Identifier ;
                         rdfs:comment "A composite identifier that has a hierarchical structure"@en ;
                         rdfs:label "CompositeIdentifier"@en .


###  https://w3id.org/def/didl#Credential
didl:Credential rdf:type owl:Class ;
                rdfs:subClassOf didl:Identity ;
                owl:disjointWith didl:Identifier ;
                rdfs:comment "A proof of an entity's identity"@en ;
                rdfs:label "Credential"@en .


###  https://w3id.org/def/didl#CredentialFormat
didl:CredentialFormat rdf:type owl:Class ;
                      owl:disjointWith didl:IdentifierFormat ;
                      rdfs:comment "A credential format that is specified by a standard or a protocol"@en ;
                      rdfs:label "CredentialFormat"@en .


###  https://w3id.org/def/didl#Identifier
didl:Identifier rdf:type owl:Class ;
                rdfs:subClassOf didl:Identity ;
                rdfs:comment "A unique reference to distinguish one entity from another"@en ;
                rdfs:label "Identifier"@en .


###  https://w3id.org/def/didl#IdentifierFormat
didl:IdentifierFormat rdf:type owl:Class ;
                      rdfs:comment "An identifier format that is specified by a standard or a protocol"@en ;
                      rdfs:label "IdentifierFormat"@en .


###  https://w3id.org/def/didl#IdentifierFunctional
didl:IdentifierFunctional rdf:type owl:Class ;
                          rdfs:comment "A concept that represents the use of  an identifier"@en ;
                          rdfs:label "IdentifierFunctional"@en .


###  https://w3id.org/def/didl#Identity
didl:Identity rdf:type owl:Class ;
              rdfs:comment "A digital identity that can be specialized to identifiers, credentials, or assertions"@en ;
              rdfs:label "Identity"@en .


###  https://w3id.org/def/didl#IdentitySubject
didl:IdentitySubject rdf:type owl:Class ;
                     rdfs:comment "An entity that is identified by an identity"@en ;
                     rdfs:label "IdentitySubject"@en .


###  https://w3id.org/def/didl#InherenceBasedCredential
didl:InherenceBasedCredential rdf:type owl:Class ;
                              rdfs:subClassOf didl:CredentialFormat ;
                              rdfs:comment "A credential that indicates something you inherently have"@en ;
                              rdfs:label "InherenceBasedCredential"@en .


###  https://w3id.org/def/didl#Key
didl:Key rdf:type owl:Class ;
         rdfs:comment "Relates to the key of an attribute's key-value pair"@en ;
         rdfs:label "Key"@en .


###  https://w3id.org/def/didl#KnowledgeBasedCredential
didl:KnowledgeBasedCredential rdf:type owl:Class ;
                              rdfs:subClassOf didl:CredentialFormat ;
                              rdfs:comment "A credential that indicates something you know"@en ;
                              rdfs:label "KnowledgeBasedCredential"@en .


###  https://w3id.org/def/didl#PossessionBasedCredential
didl:PossessionBasedCredential rdf:type owl:Class ;
                               rdfs:subClassOf didl:CredentialFormat ;
                               rdfs:comment "A credential that indicates something you have"@en ;
                               rdfs:label "PossessionBasedCredential"@en .


###  https://w3id.org/def/didl#Status
didl:Status rdf:type owl:Class ;
            rdfs:comment "Relates to the status of an identity, including active, inactive, or revoked"@en ;
            rdfs:label "Status"@en .


###  https://w3id.org/def/didl#Value
didl:Value rdf:type owl:Class ;
           rdfs:comment "Relates to the value of an attribute's key-value pair"@en ;
           rdfs:label "Value"@en .


###  https://w3id.org/security#Proof
sec:Proof rdf:type owl:Class .


###  https://www.w3.org/ns/credentials#VerifiableCredential
cred:VerifiableCredential rdf:type owl:Class .


###  https://www.w3.org/ns/credentials#VerifiablePresentation
cred:VerifiablePresentation rdf:type owl:Class .


#################################################################
#    Individuals
#################################################################

###  https://w3id.org/def/didl#AccessToken
didl:AccessToken rdf:type owl:NamedIndividual ,
                          didl:AssertionFormat ;
                 rdfs:comment "A time-bound token issued by an authorization server that grants a client application permission to access protected resources on behalf of a user or itself, see also RFC 6749"@en ;
                 rdfs:label "AccessToken" .


###  https://w3id.org/def/didl#Active
didl:Active rdf:type owl:NamedIndividual ,
                     didl:Status ;
            rdfs:comment "Active status of an identity"@en ;
            rdfs:label "Active" .


###  https://w3id.org/def/didl#Address
didl:Address rdf:type owl:NamedIndividual ,
                      didl:Key ;
             rdfs:comment "A key representing an address attribute"@en ;
             rdfs:label "Address"@en .


###  https://w3id.org/def/didl#ApplicationToken
didl:ApplicationToken rdf:type owl:NamedIndividual ,
                               didl:AssertionFormat ;
                      rdfs:comment "A token issued to an application (rather than a user) to authenticate itself when accessing APIs or services, often used in machine-to-machine (M2M) communication."@en ;
                      rdfs:label "ApplicationToken" .


###  https://w3id.org/def/didl#BearerToken
didl:BearerToken rdf:type owl:NamedIndividual ,
                          didl:AssertionFormat ;
                 rdfs:comment "A type of access token that allows access to a resource simply by presenting the token, without requiring additional proof of identity—\"whoever bears it, can use it.\""@en ;
                 rdfs:label "BearerToken" .


###  https://w3id.org/def/didl#CertificateID
didl:CertificateID rdf:type owl:NamedIndividual ,
                            didl:IdentifierFunctional ;
                   rdfs:comment "ID used in the functional scope of certificates"@en ;
                   rdfs:label "CertificateID" .


###  https://w3id.org/def/didl#ContractID
didl:ContractID rdf:type owl:NamedIndividual ,
                         didl:IdentifierFunctional ;
                rdfs:comment "ID used in the functional scope of contracts"@en ;
                rdfs:label "ContractID"@en .


###  https://w3id.org/def/didl#DID
didl:DID rdf:type owl:NamedIndividual ,
                  didl:IdentifierFormat ;
         rdfs:comment "A globally unique, cryptographically verifiable identifier that does not require a centralized registry and is designed to enable self-sovereign digital identity, see also W3C DID https://www.w3.org/TR/did-1.0/"@en ;
         rdfs:label "DID" .


###  https://w3id.org/def/didl#DN
didl:DN rdf:type owl:NamedIndividual ,
                 didl:IdentifierFormat ;
        rdfs:comment "A unique hierarchical identifier used to unambiguously identify an entry in an X.500 directory, composed of attribute–value pairs"@en ;
        rdfs:label "DN" .


###  https://w3id.org/def/didl#DateOfBirth
didl:DateOfBirth rdf:type owl:NamedIndividual ,
                          didl:Key ;
                 rdfs:comment "A key representing a date of birth attribute"@en ;
                 rdfs:label "DateOfBirth"@en .


###  https://w3id.org/def/didl#Department
didl:Department rdf:type owl:NamedIndividual ,
                         didl:Key ;
                rdfs:comment "A key representing a department attribute"@en ;
                rdfs:label "Department"@en .


###  https://w3id.org/def/didl#DeviceID
didl:DeviceID rdf:type owl:NamedIndividual ,
                       didl:IdentifierFunctional ;
              rdfs:comment "ID used in the functional scope of devices"@en ;
              rdfs:label "DeviceID" .


###  https://w3id.org/def/didl#DocumentID
didl:DocumentID rdf:type owl:NamedIndividual ,
                         didl:IdentifierFunctional ;
                rdfs:comment "ID used in the functional scope of documents"@en ;
                rdfs:label "DocumentID" .


###  https://w3id.org/def/didl#E.164
didl:E.164 rdf:type owl:NamedIndividual ,
                    didl:IdentifierFormat ;
           rdfs:comment "An ITU-T Recommendation for public telephone systems that defines the format of phone numbers, typically up to 15 digits, including country codes (e.g., +1 650 555 1234)."@en ;
           rdfs:label "E.164" .


###  https://w3id.org/def/didl#EPC
didl:EPC rdf:type owl:NamedIndividual ,
                  didl:IdentifierFormat ;
         rdfs:comment "A unique identifier designed to track individual physical objects in the supply chain using RFID technology, enabling item-level identification beyond traditional barcodes."@en ;
         rdfs:label "EPC" .


###  https://w3id.org/def/didl#EUI-48
didl:EUI-48 rdf:type owl:NamedIndividual ,
                     didl:IdentifierFormat ;
            rdfs:comment "A 48-bit globally unique identifier typically used to identify network interfaces (commonly known as a MAC address), assigned by IEEE to ensure uniqueness across devices."@en ;
            rdfs:label "EUI-48" .


###  https://w3id.org/def/didl#EUI-64
didl:EUI-64 rdf:type owl:NamedIndividual ,
                     didl:IdentifierFormat ;
            rdfs:comment "A 64-bit globally unique identifier used to identify hardware or devices, often derived from a 48-bit MAC address and used in protocols like IPv6 for interface identifiers."@en ;
            rdfs:label "EUI-64"@en .


###  https://w3id.org/def/didl#Email
didl:Email rdf:type owl:NamedIndividual ,
                    didl:Key ;
           rdfs:comment "A standardized structure for identifying electronic mailboxes, typically in the form local-part@domain, see also RFC 5322 and RFC 6531"@en ;
           rdfs:label "Email" .


###  https://w3id.org/def/didl#Fingerprint
didl:Fingerprint rdf:type owl:NamedIndividual ,
                          didl:InherenceBasedCredential ;
                 rdfs:comment "A biometric credential format that captures and encodes a person's unique fingerprint features—typically minutiae points—into a standardized digital representation for authentication or identification, see also IEC 19704-2"@en ;
                 rdfs:label "Fingerprint" .


###  https://w3id.org/def/didl#FirstName
didl:FirstName rdf:type owl:NamedIndividual ,
                        didl:Key ;
               rdfs:comment "A key representing a first name attribute"@en ;
               rdfs:label "FirstName"@en .


###  https://w3id.org/def/didl#GUID
didl:GUID rdf:type owl:NamedIndividual ,
                   didl:IdentifierFormat ;
          rdfs:comment "A 128-bit value generated using specific algorithms to ensure uniqueness across time and space, commonly used to identify objects, records, or resources in software systems."@en ;
          rdfs:label "GUID"@en .


###  https://w3id.org/def/didl#Gender
didl:Gender rdf:type owl:NamedIndividual ,
                     didl:Key ;
            rdfs:comment "A key representing a gender attribute"@en ;
            rdfs:label "Gender"@en .


###  https://w3id.org/def/didl#IDToken
didl:IDToken rdf:type owl:NamedIndividual ,
                      didl:AssertionFormat ;
             rdfs:comment "A security token issued by an OpenID Connect Provider that contains claims about the authentication of an end-user and possibly their identity attributes, typically formatted as a signed JWT."@en ;
             rdfs:label "IDToken"@en .


###  https://w3id.org/def/didl#IRI
didl:IRI rdf:type owl:NamedIndividual ,
                  didl:IdentifierFormat ;
         rdfs:comment "An extended version of a URI that allows the use of Unicode characters from the Universal Character Set (UCS), enabling identifiers in languages beyond ASCII."@en ;
         rdfs:label "IRI"@en .


###  https://w3id.org/def/didl#InContract
didl:InContract rdf:type owl:NamedIndividual ,
                         didl:Key ;
                rdfs:comment "A key representing an in-contract attribute"@en ;
                rdfs:label "InContract"@en .


###  https://w3id.org/def/didl#InOrganization
didl:InOrganization rdf:type owl:NamedIndividual ,
                             didl:Key ;
                    rdfs:comment "A key representing an in-organization attribute"@en ;
                    rdfs:label "InOrganization"@en .


###  https://w3id.org/def/didl#Inactive
didl:Inactive rdf:type owl:NamedIndividual ,
                       didl:Status ;
              rdfs:comment "Inactive status of an identity"@en ;
              rdfs:label "Inactive"@en .


###  https://w3id.org/def/didl#JsonWebToken
didl:JsonWebToken rdf:type owl:NamedIndividual ,
                           didl:AssertionFormat ;
                  rdfs:comment "A compact, URL-safe token format that represents claims between parties using a JSON object, digitally signed (and optionally encrypted) for secure transmission and verification."@en ;
                  rdfs:label "JsonWebToken"@en .


###  https://w3id.org/def/didl#KerberosTicket
didl:KerberosTicket rdf:type owl:NamedIndividual ,
                             didl:AssertionFormat ;
                    rdfs:comment "A time-limited, encrypted credential issued by a Kerberos Key Distribution Center (KDC) that allows a client to authenticate to services without repeatedly sending passwords."@en ;
                    rdfs:label "KerberosTicket"@en .


###  https://w3id.org/def/didl#LastLogin
didl:LastLogin rdf:type owl:NamedIndividual ,
                        didl:Key ;
               rdfs:comment "A key representing a last login attribute"@en ;
               rdfs:label "LastLogin"@en .


###  https://w3id.org/def/didl#LastName
didl:LastName rdf:type owl:NamedIndividual ,
                       didl:Key ;
              rdfs:comment "A key representing a last name attribute"@en ;
              rdfs:label "LastName"@en .


###  https://w3id.org/def/didl#MachineID
didl:MachineID rdf:type owl:NamedIndividual ,
                        didl:IdentifierFunctional ;
               rdfs:comment "ID used as functional scope of machines"@en ;
               rdfs:label "MachineID"@en .


###  https://w3id.org/def/didl#Nationality
didl:Nationality rdf:type owl:NamedIndividual ,
                          didl:Key ;
                 rdfs:comment "A key representing a nationality attribute"@en ;
                 rdfs:label "Nationality"@en .


###  https://w3id.org/def/didl#OneTimePassword
didl:OneTimePassword rdf:type owl:NamedIndividual ,
                              didl:KnowledgeBasedCredential ;
                     rdfs:comment "A password that is valid for only one login session or transaction, typically generated dynamically and used to enhance security by preventing replay attacks."@en ;
                     rdfs:label "OneTimePassword"@en .


###  https://w3id.org/def/didl#OrganizationID
didl:OrganizationID rdf:type owl:NamedIndividual ,
                             didl:IdentifierFunctional ;
                    rdfs:comment "ID used as functional scope of organizations"@en ;
                    rdfs:label "OrganizationID"@en .


###  https://w3id.org/def/didl#Password
didl:Password rdf:type owl:NamedIndividual ,
                       didl:Key ;
              rdfs:comment "A key representing a password attribute"@en ;
              rdfs:label "Password"@en .


###  https://w3id.org/def/didl#PasswordCredential
didl:PasswordCredential rdf:type owl:NamedIndividual ,
                                 didl:KnowledgeBasedCredential ;
                        rdfs:comment "This refers to password credentials, always combined with a username"@en ;
                        rdfs:label "PasswordCredential"@en .


###  https://w3id.org/def/didl#PhoneNumber
didl:PhoneNumber rdf:type owl:NamedIndividual ,
                          didl:Key ;
                 rdfs:comment "A key representing a phone number attribute"@en ;
                 rdfs:label "PhoneNumber"@en .


###  https://w3id.org/def/didl#ProcessID
didl:ProcessID rdf:type owl:NamedIndividual ,
                        didl:IdentifierFunctional ;
               rdfs:comment "ID used as functional scope of a process"@en ;
               rdfs:label "ProcessID"@en .


###  https://w3id.org/def/didl#ProductID
didl:ProductID rdf:type owl:NamedIndividual ,
                        didl:IdentifierFunctional ;
               rdfs:comment "ID used as functional scope of a product"@en ;
               rdfs:label "ProductID"@en .


###  https://w3id.org/def/didl#PublicKey
didl:PublicKey rdf:type owl:NamedIndividual ,
                        didl:Key ;
               rdfs:comment "A key representing a public key attribute"@en ;
               rdfs:label "PublicKey"@en .


###  https://w3id.org/def/didl#RFC1035
didl:RFC1035 rdf:type owl:NamedIndividual ,
                      didl:IdentifierFormat ;
             rdfs:comment "A foundational standard that specifies the implementation of the Domain Name System (DNS) — detailing message formats, query/response interactions, and resource records used for translating domain names to IP addresses."@en ;
             rdfs:label "RFC1035" .


###  https://w3id.org/def/didl#RFC5322
didl:RFC5322 rdf:type owl:NamedIndividual ,
                      didl:IdentifierFormat ;
             rdfs:comment "A standardized structure for identifying electronic mailboxes, typically in the form local-part@domain"@en ;
             rdfs:label "RFC5322"@en .


###  https://w3id.org/def/didl#RFC7613
didl:RFC7613 rdf:type owl:NamedIndividual ,
                      didl:IdentifierFormat ;
             rdfs:comment "A standard that defines rules for the precise comparison of internationalized usernames and passwords, specifying string preparation, normalization, and case-mapping to avoid ambiguities and spoofing in authentication systems."@en ;
             rdfs:label "RFC7613"@en .


###  https://w3id.org/def/didl#RefreshToken
didl:RefreshToken rdf:type owl:NamedIndividual ,
                           didl:AssertionFormat ;
                  rdfs:comment "A credential issued by an authorization server that allows a client to obtain a new access token without requiring the user to reauthenticate, typically used in long-lived sessions."@en ;
                  rdfs:label "RefreshToken"@en .


###  https://w3id.org/def/didl#ResourceID
didl:ResourceID rdf:type owl:NamedIndividual ,
                         didl:IdentifierFunctional ;
                rdfs:comment "ID used as functional scope of resources"@en ;
                rdfs:label "ResourceID"@en .


###  https://w3id.org/def/didl#Revoked
didl:Revoked rdf:type owl:NamedIndividual ,
                      didl:Status ;
             rdfs:comment "Revoked status of an identity"@en ;
             rdfs:label "Revoked"@en .


###  https://w3id.org/def/didl#Role
didl:Role rdf:type owl:NamedIndividual ,
                   didl:Key ;
          rdfs:comment "A key representing a role attribute"@en ;
          rdfs:label "Role"@en .


###  https://w3id.org/def/didl#SAML2.0Assertion
didl:SAML2.0Assertion rdf:type owl:NamedIndividual ,
                               didl:AssertionFormat ;
                      rdfs:comment "A structured XML statement issued by an Identity Provider (IdP) in a SAML 2.0 authentication exchange, containing claims (such as user identity, authentication status, and attributes) that a Service Provider (SP) can trust."@en ;
                      rdfs:label "SAML2.0Assertion"@en .


###  https://w3id.org/def/didl#SerialNumber
didl:SerialNumber rdf:type owl:NamedIndividual ,
                           didl:Key ;
                  rdfs:comment "A key representing a serial number attribute"@en ;
                  rdfs:label "SerialNumber"@en .


###  https://w3id.org/def/didl#SessionKey
didl:SessionKey rdf:type owl:NamedIndividual ,
                         didl:PossessionBasedCredential ;
                rdfs:comment "A session-based key as a credential used for temporary authentication"@en ;
                rdfs:label "SessionKey"@en .


###  https://w3id.org/def/didl#Signature
didl:Signature rdf:type owl:NamedIndividual ,
                        didl:PossessionBasedCredential ;
               rdfs:comment "A cryptographic proof—typically a digital signature—used to validate the authenticity and integrity of a credential or assertion, often embedded in formats like JWTs, SAML assertions, or verifiable credentials."@en ;
               rdfs:label "Signature"@en .


###  https://w3id.org/def/didl#SmartCard
didl:SmartCard rdf:type owl:NamedIndividual ,
                        didl:PossessionBasedCredential ;
               rdfs:comment "A physical card with embedded integrated circuits capable of securely storing and processing data—often used for authentication, digital signatures, and secure credential storage in identity systems."@en ;
               rdfs:label "SmartCard"@en .


###  https://w3id.org/def/didl#Title
didl:Title rdf:type owl:NamedIndividual ,
                    didl:Key ;
           rdfs:comment "A key representing a title attribute"@en ;
           rdfs:label "Title"@en .


###  https://w3id.org/def/didl#URI
didl:URI rdf:type owl:NamedIndividual ,
                  didl:IdentifierFormat ;
         rdfs:comment "A standardized string used to uniquely identify a resource on the Internet or a private network, encompassing both URLs and URNs."@en ;
         rdfs:label "URI"@en .


###  https://w3id.org/def/didl#URL
didl:URL rdf:type owl:NamedIndividual ,
                  didl:IdentifierFormat ;
         rdfs:comment "A type of URI that not only identifies a resource but also provides a means of locating it by describing its access mechanism (e.g., https, ftp) and network location."@en ;
         rdfs:label "URL"@en .


###  https://w3id.org/def/didl#URN
didl:URN rdf:type owl:NamedIndividual ,
                  didl:IdentifierFormat ;
         rdfs:comment "A type of URI intended to serve as a persistent, location-independent resource identifier, often used to name resources in a globally unique and stable way (e.g., urn:isbn:0451450523)."@en ;
         rdfs:label "URN"@en .


###  https://w3id.org/def/didl#UUIDv1
didl:UUIDv1 rdf:type owl:NamedIndividual ,
                     didl:IdentifierFormat ;
            rdfs:comment "Time-based UUID"@en ;
            rdfs:label "UUIDv1"@en .


###  https://w3id.org/def/didl#UUIDv2
didl:UUIDv2 rdf:type owl:NamedIndividual ,
                     didl:IdentifierFormat ;
            rdfs:comment "Distributed Computing Environment (DCE) Security UUID"@en ;
            rdfs:label "UUIDv2"@en .


###  https://w3id.org/def/didl#UUIDv3
didl:UUIDv3 rdf:type owl:NamedIndividual ,
                     didl:IdentifierFormat ;
            rdfs:comment "Name-based UUID using MD5"@en ;
            rdfs:label "UUIDv3"@en .


###  https://w3id.org/def/didl#UUIDv4
didl:UUIDv4 rdf:type owl:NamedIndividual ,
                     didl:IdentifierFormat ;
            rdfs:comment "Random UUID with no embedded metadata, offering a high degree of uniqueness"@en ;
            rdfs:label "UUIDv4"@en .


###  https://w3id.org/def/didl#UUIDv5
didl:UUIDv5 rdf:type owl:NamedIndividual ,
                     didl:IdentifierFormat ;
            rdfs:comment "Name-based UUID using SHA-1"@en ;
            rdfs:label "UUIDv5"@en .


###  https://w3id.org/def/didl#UserID
didl:UserID rdf:type owl:NamedIndividual ,
                     didl:IdentifierFunctional ;
            rdfs:comment "ID used as functional scope of human users"@en ;
            rdfs:label "UserID"@en .


###  https://w3id.org/def/didl#Username
didl:Username rdf:type owl:NamedIndividual ,
                       didl:Key ;
              rdfs:comment "A key representing a username attribute"@en ;
              rdfs:label "Username"@en .


###  https://w3id.org/def/didl#VerifiableCredential
didl:VerifiableCredential rdf:type owl:NamedIndividual ,
                                   didl:AssertionFormat ,
                                   cred:VerifiableCredential ;
                          rdfs:comment "A tamper-evident digital credential containing claims about a subject, cryptographically signed by an issuer, and compliant with a standard format for decentralized identity ecosystems."@en ;
                          rdfs:label "VerifiableCredential"@en .


###  https://w3id.org/def/didl#VerifiablePresentation
didl:VerifiablePresentation rdf:type owl:NamedIndividual ,
                                     didl:AssertionFormat ,
                                     cred:VerifiablePresentation ;
                            rdfs:comment "A packaged set of one or more Verifiable Credentials shared by a holder with a verifier, optionally including selective disclosure and proofs of authenticity."@en ;
                            rdfs:label "VerifiablePresentation"@en .


###  https://w3id.org/def/didl#Voice
didl:Voice rdf:type owl:NamedIndividual ,
                    didl:InherenceBasedCredential ;
           rdfs:comment "A biometric credential format that encodes the unique vocal characteristics of a person—such as pitch, tone, and rhythm—into a digital template for speaker verification or identification."@en ;
           rdfs:label "Voice"@en .


###  https://w3id.org/def/didl#X.509Certificate
didl:X.509Certificate rdf:type owl:NamedIndividual ,
                               didl:AssertionFormat ;
                      rdfs:comment "A digital certificate that uses the X.509 public key infrastructure (PKI) standard to bind a subject's identity to a public key, and is signed by a trusted Certificate Authority (CA)."@en ;
                      rdfs:label "X.509Certificate"@en .


###  Generated by the OWL API (version 4.5.29.2024-05-13T12:11:03Z) https://github.com/owlcs/owlapi
